ulib/LowStar.Array.Modifies.fsti
@@ -609,10 +609,14 @@ val loc_union_gsub (#a:Type0) (b:array a) (i len1 len2:U32.t)
          (ensures loc_union (loc_array (gsub b i len1)) (loc_array (gsub b (i `U32.add` len1) len2))
                   == loc_array (gsub b i (len1 `U32.add` len2)))
 
+
+val loc_union_is_split_into (#a: Type) (b b1 b2: array a) : Lemma
+  (requires (is_split_into b (b1, b2)))
+  (ensures (loc_array b == loc_array b1 `loc_union` loc_array b2))
+
 val disjoint_gsubs (#a:Type0) (b:array a) (i1 i2:U32.t) (len1:U32.t{U32.v len1 > 0}) (len2:U32.t{U32.v len2 > 0})
   :Lemma (requires (UInt32.v i1 + UInt32.v len1 <= (vlength b) /\
                     UInt32.v i2 + UInt32.v len2 <= (vlength b) /\
 		    (UInt32.v i1 + UInt32.v len1 <= UInt32.v i2 \/
                      UInt32.v i2 + UInt32.v len2 <= UInt32.v i1)))
          (ensures  (loc_disjoint (loc_array (gsub b i1 len1)) (loc_array (gsub b i2 len2))))
-  
